When we were solving for bessel's functions, we took the differential equation by frobenius and assumed a solution of the form

$$
\begin{align}
y(x)= \sum_{k=0}^{\infty} a_{k}x^{k+l}
\end{align}
$$
where $l$ is some number.

$$
\begin{align}
\sum_{k=0}^{\infty} \left\{ a_{k}[(k+l)^{2}-n^{2}]+a_{k-1} \right\}x^{k+l} =0 
\end{align}
$$
We take $a_{0}$=1. For every power of $x$ we have to get zero, so $(0+l)^{2}-n^{2}=0$.

This implies that $l=\pm n$.
$a_{1}[(1+l)^{2}-n^{2}]=0$, which we can stuff in the $l$ to get
$$
\begin{align}
a_{1}[(1\pm  n^{2})-n^{2}]=0 \\
a_{1}(1\pm  2n)=0
\end{align}
$$
This is sufficient to prove that $a_{1}$ must be zero. 


Look up newtons heat equation. We reduce that to an equation saying
net power in = source power - heat flow in + heat flow out.

We get the heat equation
$$
\begin{align}
c\rho \frac{ \partial u }{ \partial t } - \frac{ \partial  }{ \partial x } \left( \kappa \frac{ \partial u }{ \partial x }  \right) = g(x,t)
\end{align}
$$


![[20250408_103002.jpg]]


The Schr√∂dinger equation becomes the diffusion equation if you use an imaginary time. 


