## 6.6.4
Find the matrix $[T]_{C \leftarrow B}$ of the linear transformation $T: V \to W$ with respect to the bases $\mathcal{B}$ and $\mathcal{C}$ of $V$ and $W$, respectively. Verify Theorem 6.26 for the vector $\mathbf{v}$ by computing $T(\mathbf{v})$ directly and using the theorem.

Let $T: \mathscr{P}_2 \to \mathscr{P}_2$ be defined by $T( p(x) ) = p(x+2)$, let $\mathcal{B} = \{1, x+2, (x+2)^2\}$, $\mathcal{C} = \{1, x, x^2\}$, and $\mathbf{v} = p(x) = a+bx+cx^2$
![[Pasted image 20240415193523.png]]
First, I compute

$T(v_{1})=T(1)=1$
$T(v_{2})=T(x+2)=(x+2)+2 = x+4$ $T(v_{3})=T((x+2))^{2}=((x+2)+2)^{2}=(x+4)^{2}=x^{2}+8x+16$
Writing these out in $c$ yields
$$
[T(v_{1})]_{c}=\begin{pmatrix}
0 \\ 0 \\ 1
\end{pmatrix}, [T(v_{2})]_{c} = \begin{pmatrix}
0 \\ 1 \\ 4
\end{pmatrix}, [T(v_{3})]_{c} = \begin{pmatrix}
1 \\ 8 \\ 16
\end{pmatrix}
$$

Therefore the matrix of $T$ with respect to $\mathcal{B} \text{ and } \mathcal{C}$ is
$$
\begin{align}
A=[T]_{c\leftarrow  b}=[[T(v_{1})]_{c} [T(v_{2})]_{c} [T(v_{3})]_{c}] \\
= \begin{bmatrix}
0 & 0 & 1 \\
0 & 1 & 8 \\
1 & 4 & 16
\end{bmatrix}
\end{align}
$$
We can verify theorem 6.26. First, I compute
$$
\begin{align}
T(v)&=T(a+bx+cx^{2}) \\
&= a+b(x+2)+c(x+2)^{2} \\
&= a+bx+2b+c(x^{2}42x+4) \\
&= a+bx+2b+cx^{2}+4cx+4c \\
T(v)&=(a+2b+4c)+(b+4c)x+cx^{2}
\end{align}
$$


Now, I compute $[v]_{\mathcal{B}}$
$$
\begin{align}
\mathcal{B} &= \{1, x+2, (x+2)^2\}  \\
\mathcal{B} &= \{1, x+2, x^{2}+4x+4\}  \\
\mathcal{B} &= \begin{bmatrix}
0 & 0 & 1 \\
0 & 1 & 4 \\
1 & 2 & 4
\end{bmatrix}
\end{align}
$$
We can now find $V$ in B by
$$
\begin{align}
a+bx+cx^{2}=c_{1}+c_{2}(x+2)+c_{3}(x^{2}+4x+4) \\ \\
\begin{bmatrix}
c_{1} & 2c_{2} & 4c_{3} & | & a \\
0 & c_{2} & 4c_{3} & | & b \\
0 & 0 & c_{3} & | & c
\end{bmatrix} \\
\begin{bmatrix}
1 & 2 & 4 & | & a \\
0 & 1 & 4 & | & b \\
0 & 0 & 1 & | & c
\end{bmatrix}
\end{align}
$$
This simplifies to
$$
\begin{align}
\begin{bmatrix}
1 & 2 & 0 & | & a-4c \\
0 & 1 & 0 & | & b-4c \\
0 & 0 & 1 & | & c
\end{bmatrix} \rightarrow  \begin{bmatrix}
1 & 0 & 0 & | & a-4c-2b+8c \\
0 & 1 & 0 & | & b-4c \\
0 & 0 & 1 & | & c
\end{bmatrix}

\end{align}
$$
This gets us $V$ in $B$ as
$$
\begin{align}
\begin{pmatrix}
a+4c-2b \\
b-4c \\
c\\
\end{pmatrix}
\end{align}
$$



Using these facts, I can now confirm that
$$
\begin{align}
 {T(v)}_{c}& =A[v]_{b}   \\
&=  \begin{bmatrix}
0 & 0 & 1 \\
0 & 1 & 8 \\
1 & 4 & 16
\end{bmatrix}
\begin{pmatrix}
a-2b+4c \\
b-4c \\
c\\
\end{pmatrix} \\
&= cx^{2}+(b-4c+8c)x+(a-2b+4c+4b-16c+16c) \\ 
(a+2b+4c)+(b+4c)x+cx^{2} &= cx^{2}+(b-4c+8c)x+(a+2b+4c) \\
\end{align}
$$


## 6.6.12
Find the matrix $[T]_{C \leftarrow B}$ of the linear transformation $T: V \to W$ with respect to the bases $\mathcal{B}$ and $\mathcal{C}$ of $V$ and $W$, respectively. Verify Theorem 6.26 for the vector $\mathbf{v}$ by computing $T(\mathbf{v})$ directly and using the theorem.

Let $T: M_{22} \to M_{22}$ be defined by $T(A) = A - A^T$, let $\mathcal{B} = \mathcal{C} = \{E_{11}, E_{12}, E_{21}, E_{22}\}$, and let $\mathbf{v} = A = \begin{bmatrix*} a & b \\ c & d \end{bmatrix*}$.

First, I will compute
$$
\begin{align}
T(E_{1,1}), T(E_{1,2}),T(E_{2,1}), T(E_{2,2})
\end{align}
$$
$$
\begin{align}
T(E_{1,1})=\begin{bmatrix}
1  & 0 \\
0 & 0
\end{bmatrix}- \begin{bmatrix}
1 & 0 \\
0 & 0
\end{bmatrix} = \begin{bmatrix}
0 & 0 \\ 0 & 0
\end{bmatrix} \\
\end{align}
$$
$$
\begin{align}
T(E_{1,2})= \begin{bmatrix}
0  & 1 \\ 0  &  0
\end{bmatrix} - \begin{bmatrix}
0 & 0 \\ 1  & 0
\end{bmatrix} = \begin{bmatrix}
0 & 1 \\ -1  & 0
\end{bmatrix} \\
\end{align}
$$

$$
\begin{align}
T(E_{2,1})= \begin{bmatrix}
0  & 0 \\ 1  &  0
\end{bmatrix} - \begin{bmatrix}
0& 1 \\ 0  & 0
\end{bmatrix} = \begin{bmatrix}
0 & -1 \\ 1  & 0
\end{bmatrix}  \\
\end{align}
$$

$$
\begin{align}
T(E_{2,2})= \begin{bmatrix}
0  & 0 \\ 0  &  1
\end{bmatrix} - \begin{bmatrix}
0 & 0 \\ 0  & 1
\end{bmatrix} = \begin{bmatrix}
0 & 0 \\ 0 & 0
\end{bmatrix} \\
\end{align}
$$
This gives us our matrix for the transformation, as $\mathcal{B}\text{ and } \mathcal{C}$ have the same basis.
The transformation matrix multiplies each transformed basis matrix the corresponding value in the matrix we want to act on. 
$$
\begin{align}
0_{2\times  2}, \begin{bmatrix}
0&1\\-1&0
\end{bmatrix},  \begin{bmatrix}
0&-1\\1&0
\end{bmatrix},  0_{2\times  2}
\end{align}
$$

Using the theorem, this means that out matrix would be
$$
\begin{align} 
a\begin{bmatrix}
\vec{0}
\end{bmatrix} + b \begin{bmatrix}
0 & 1 \\
-1 & 0
\end{bmatrix}+c \begin{bmatrix}
0 & -1 \\
1 & 0
\end{bmatrix}+d\begin{bmatrix}
\vec{0}
\end{bmatrix} \\
= \begin{bmatrix}
0 & b-c \\
c- b & 0
\end{bmatrix}
\end{align}
$$
We can also compute directly, 
$$
\begin{align}
T\left( \begin{bmatrix}
a  & b \\ c & d
\end{bmatrix} \right) =\begin{bmatrix}
a  & b \\ c & d
\end{bmatrix}-\begin{bmatrix}
a  & c \\ b & d
\end{bmatrix} \\
= \begin{bmatrix}
0  & b-c \\
c-b & 0
\end{bmatrix}
\end{align}
$$

We see that computing by each component of the basis vs computing directly reached the same answer, so the theorem holds true for this example.


## 6.6.14

Consider the subspace $W$ of $\mathscr{D}$ given by $W = \text{span}(e^{2x}, e^{-2x})$.

Show that the differential operator $D$ maps $W$ into itself
By applying The differential operator onto the original basis, we can find a transformed basis for the output of the differential operator. 
Directly computing, 
$$
\begin{align}
\frac{d}{dx}e^{2x}&=2e^{2x} \\
\frac{d}{dx} e^{-2x}&=-2e^{-2x}
\end{align}
$$
This gives us a basis for the output space as
$$
\begin{align}
2e^{2x},-2e^{ -2x }
\end{align}
$$
We can see that this these are linear combinations of the original basis: $v_{1}$ was multiplied by 2 and $v_{2}$ was multiplied by -2. Thus, The differential operator has mapped the basis from $W$ into a scaled version of that basis in $W$. Thus, $D$ maps a scaled version of the space of $W$ onto itself.



Find the matrix of $D$ with respect to $\mathcal{B} = \{e^{2x}, e^{-2x}\}$.
The differential operator acting on this set yields the output
$$
\begin{align}
\left\{ 2e^{ 2x },-2e^{ -2x } \right\}
\end{align}
$$
Which is 
$$
\begin{align}
\left\{ \begin{bmatrix}
2 \\ 0 
\end{bmatrix} , \begin{bmatrix}
0 \\ -2
\end{bmatrix} 
 \right\}
\end{align}
$$
We can write this as the matrix
$$
\begin{align}
D=\begin{bmatrix}
2 & 0 \\
0 &  -2 \\
\end{bmatrix}
\end{align}
$$



Compute the derivative of $f(x) = e^{2x}-3e^{-2x}$ indirectly, using Theorem 6.26, and verify that it agrees with $f'(x)$ as computed directly.

Computing directly, we get:
$$
\begin{align}
f'(x)=2e^{2x} +6e^{-2x}
\end{align}
$$
We can also use the matrix for $D$ with
$$
\begin{align}
\begin{bmatrix}
2 & 0\\
0 & -2 
\end{bmatrix} \begin{pmatrix}
2 \\ 6
\end{pmatrix} = 4v_{1}-12v_{2} \\
= 4e^{2x}-12e^{-2x} \\
\end{align}
$$
We can see that this produced the same output, so our differential operator matrix works.


## 6.6.16
Consider the subspace $W$ of $\mathscr{D}$ given by $W = \text{span}(\text{cos}(x), \text{sin}(x), x\text{cos}(x), x\text{sin}(x))$.
Find the matrix of $D$ with respect to $\mathcal{B} = \{\text{cos}(x), \text{sin}(x), x\text{cos}(x), x\text{sin}(x)\}$.

Assuming $D$ is the differential operator, then
I compute $D$ on every element of the basis $\mathcal{B}$
$$
\begin{align}
D(\cos x)&=-\sin x \\
D(\sin(x))&=\cos x \\
D(x\cos x)&=-x\sin x+\cos x \\
D(x\sin x)&=x\cos x+\sin x
\end{align}
$$
We can represent this in terms of the original basis $\mathcal{B}$ as
$$
\begin{align}
\begin{pmatrix}
0\\-1\\0\\0 
\end{pmatrix},\begin{pmatrix}
1\\0\\0\\0
\end{pmatrix},\begin{pmatrix}
1\\0\\0\\-1
\end{pmatrix},
\begin{pmatrix}
0\\1\\1\\0
\end{pmatrix}
\end{align}
$$
This gives us the matrix for the transformation as
$$
\begin{align}
\begin{bmatrix}
0 & 1 & 1 & 0 \\
-1 & 0 & 0 & 1 \\
0 & 0 & 0 & 1 \\
0 & 0 & -1 & 0
\end{bmatrix}
\end{align}
$$


Compute the derivative of $f(x) = \text{cos}(x)+2x\text{cos}(x)$ indirectly, using Theorem 6.26, and verify that it agrees with $f'(x)$ as computed directly.

Computing directly yields:
$$
\begin{align}
-\sin x-2x\sin x+2\cos x
\end{align}
$$

$$
\begin{align}
f(x)\text{ in the basis is } \begin{pmatrix}
1 \\ 0 \\ 2 \\ 0
\end{pmatrix}
\end{align}
$$
Thus, we can compute the differential operator with
$$
\begin{align}
\begin{bmatrix}
0 & 1 & 1 & 0 \\
-1 & 0 & 0 & 1 \\
0 & 0 & 0 & 1 \\
0 & 0 & -1 & 0
\end{bmatrix}\begin{pmatrix}
1 \\ 0 \\ 2 \\ 0
\end{pmatrix}=\begin{pmatrix}
2 \\ -1 \\ 0 \\ -2
\end{pmatrix}
\end{align}
$$

which is equal to
$$
\begin{align}
2\cos(x) -\sin(x) -2x\sin(x) 
\end{align}
$$
This agrees with direct computation, so the matrix is correct. 

## 6.6.22
Determine whether the linear transformation $T$ is invertible by considering its matrix with respect to the standard bases. If $T$ is invertible, use Theorem 6.28 and the method of Example 6.82 to find $T^{-1}$.
$$
T: \mathscr{P}_2 \to \mathscr{P}_2 \text{ defined by } T(p(x)) = p'(x)
    
$$

The linear transformation is not invertible, as all constants are taken to the null space zero.
If we have a vector $a+bx+cx^{2}$, the differential operator yields $b+2cx$. 
We can take the basis $\left\{ 1,x,x^{2} \right\}$ and apply the differential to generate the matrix:
$T(1)=0,T(x)=1, T(x^{2})=2x$
Writing this output in the initial basis yields the transformation matrix
$$
\begin{align}
\begin{bmatrix}
0 &  1&  0\\
0 &  0&  2\\
0 &  0& 0 \\
\end{bmatrix}
\end{align}
$$
We can see that this has a null space corresponding to every constant. Having a null space other than the trivial solution means that a transformation is not invertible.
## 7.1.2
Let
$$
\mathbf{u} = \begin{bmatrix*}[r] 1 \\ -2 \end{bmatrix*} \ \ \ \text{and} \ \ \ 
\mathbf{v} = \begin{bmatrix*}[r] 4 \\ 3 \end{bmatrix*}. 
$$
Let $\langle\mathbf{u},\mathbf{v}\rangle$ be the inner product of Example 7.3, with $A = \begin{bmatrix*}[r] 6 & 2 \\ 2 & 3 \end{bmatrix*}$. Compute

\item[(a)] $\langle\mathbf{u},\mathbf{v}\rangle$
$$
\begin{align}
\left< u,v \right> =u^{T}Av \\
= [1 ,-2 ]  \begin{bmatrix}
6 & 2 \\
2 & 3
\end{bmatrix} \begin{bmatrix}
4 \\ 3
\end{bmatrix} \\
= 6*1*4+2*1*3+2*-2*4+3*-2*3 \\
=24+6 -16 -18 \\
= -4
\end{align}
$$

\item[(b)] $\lVert \mathbf{u} \rVert$
Using our version of the inner product,
$$
\begin{align}
\left< u,u \right>& = u^{T}Au \\
&= [1,-2] \begin{bmatrix}
6 & 2 \\ 2 & 3
\end{bmatrix} \begin{bmatrix}
1 \\ -2
\end{bmatrix} \\
&=[1,-2]\begin{bmatrix}
2 \\ -4
\end{bmatrix} \\
&=2+8 \\
&=10
\end{align}
$$



\item[(c)] $\text{d}(\mathbf{u},\mathbf{v})$


$$
\begin{align}
d(u,v)&=\lvert u-v \rvert=\sqrt{ \left< u-v,u-v \right> }\rvert \\
&= \sqrt{[-3,-5] \begin{bmatrix}
6 & 2 \\ 2 & 3
\end{bmatrix}\begin{bmatrix}
-3\\-5
\end{bmatrix} }
\end{align}
$$
$$
\begin{align}
\sqrt{ [-3,-5]\begin{bmatrix}
-28\\-21
\end{bmatrix} } \\
=\sqrt{ 84+105  }\\
=\sqrt{ 189 }
\end{align}
$$


## 7.1.4
 In Exercise 7.1.2, find a nonzero vector orthogonal to $\mathbf{u}$.
 $$
\begin{align}
u=\begin{bmatrix}
1\\-2
\end{bmatrix}
\end{align}
$$
A vector orthogonal to $u$ satisfies
$$
\begin{align}
\left< u,v \right> =0 \\
[1,-2]\begin{bmatrix}
6 & 2\\2 & 3
\end{bmatrix} \begin{bmatrix}
v_{1}\\v_{2}
\end{bmatrix} \\
[1,-2]\begin{bmatrix}
6v_{1}+2v_{2}\\2v_{1}+3v_{2}
\end{bmatrix} \\
0=6v_{1}+2v_{2}-4v_{1}-6v_{2} \\
0=2v_{1}-4v_{2}
\end{align}
$$
Choosing  $v_{2}=1$
$$
\begin{align}
v_{1}=2
\end{align}
$$
This gives $v=\begin{bmatrix}2\\1\end{bmatrix}$ is orthogonal to $\begin{bmatrix}1\\-2\end{bmatrix}$




## 7.1.6
Let $\langle p(x),q(x)\rangle$ be the inner product of Example 7.5 on the vector space $\mathscr{P}_2[0, 1]$. Let $p(x) = 3 - 2x$ and $q = 1 + x + x^2$. Compute
\item[(a)] $\langle p(x),q(x)\rangle$

using the definition from $7.5$ yields
$$
\begin{align}
\left< p(x),q(x) \right> &= \int_{0}^{1} (3-2x)(1+x+x^{2}) \, dx  \\
&=\int_{0}^{1} -2x^{3}+x^{2}+x+3 \, dx \\
&=\left( -\frac{1}{2}x^{4}+\frac{x^{3}}{3}+\frac{x^{2}}{2}+3x \right)\bigg|_{0}^{1} \\
&=\left( -\frac{1}{2}+\frac{1}{3}+\frac{1}{2}+3 \right)    \\
&=\frac{10}{3}
\end{align}
$$

\item[(b)] $\lVert p(x) \rVert$
$$
\begin{align}
\left< p(x),p(x) \right> &=\int_{0}^{1} (3-2x)^{2} \, dx  \\
\int_{0}^{1} 9 -12x+4x^{2}\, dx  \\
=\left( 9x-6x^{2}+\frac{4}{3}x^{3} \right) \bigg|_{0}^{1} \\
=\left( 9-6+\frac{4}{3} \right)    \\
 \\
\left| p(x)  \right|=\sqrt{ \left< p(x),p(x) \right>  }=\sqrt{ \frac{13}{3} }
\end{align}
$$

\item[(c)] $\text{d}(p(x),q(x))$
$$
\begin{align}
\left< p(x)-q(x),p(x)-q(x) \right> &=\int_{0}^{1} \left( (3 - 2x)-(1 + x + x^2) \right)^{2}  \, dx  \\
 &=\int_{0}^{1} \left(2 - 3x - x^2 \right)^{2} \\
 & =\int_{0}^{1}x^{4}+6x^{3}+5x^{2}-12x+4  \, dx  \\
&=\frac{x^{5}}{5}+\frac{6}{4}x^{4}+\frac{5}{3}x^{3}-6x^{2}+4x \bigg|_{0}^{1}  \\
&=\frac{1}{5}+\frac{3}{2}+\frac{5}{3}-6+4 \\
&= \frac{41}{30}

\end{align}
$$

## 7.1.8
In Exercise 7.1.6, find a nonzero vector orthogonal to $p(x)$.
To find a vector orthogonal to p(x), the vector must satisfy
$$
\begin{align}
\left< p(x),v(x) \right> &=0 \\
0&=\int_{0}^{1}  (3-2x)(v_{1}+v_{2}x+ v_{3}x^{2})\, dx  \\
0 &=\int_{0}^{1} (3-2x)v_{1}+(3-2x)v_{2}x+(3-2x)v_{3}x^{2} \\
0 & =\int_{0}^{1}3v_{1}-2xv_{1} +3v_{2}x-2v_{2}x^{2}+3v_{3}-2v_{3}x^{3}  \, dx  \\
0 & =\int_{0}^{1} -2v_{3}x^{3}-2v_{2}x^{2}+3v_{3}x^{2}-2v_{1}x+3v_{2}x+3v_{1} \, dx  \\
 & = \int_{0}^{1} (-2v_{3})x^{3}+(-2v_{2}+3v_{3})x^{2} + (-2v_{1}+3v_{2})x+3v_{1} \, dx \\
 & =\left( -\frac{1}{2}v_{3}-\frac{2}{3}v_{2}+v_{3}-v_{1}+\frac{3}{2}v_{2}+3v_{1} \right)  \\
\end{align}
$$
$$
\begin{align}
0 & =  -\frac{5}{6}v_{2}+\frac{v_{3}}{2}-v_{1}+3v_{1}\\
\end{align}
$$
Choosing an arbitrary $v_{1},v_{2}:v_{1}=1,v_{2}=1$
$$
\begin{align}
0=-\frac{5}{6}+\frac{v_{3}}{2}+3 \\
-\frac{13}{6} & =\frac{v_{3}}{2} \\
v_{3}=\frac{13}{3}
\end{align}
$$
This gives the orthogonal vector in $\mathscr{P}_{2}$
$$
\begin{align}
1+x+\frac{13}{3}x^{2}
\end{align}
$$



## 7.1.26
Suppose that $\mathbf{u}$, $\mathbf{v}$, and $\mathbf{w}$ are vectors in an inner product space such that 
$$

\langle \mathbf{u}, \mathbf{v} \rangle = 1, \ \ \ \ \langle \mathbf{u}, \mathbf{w} \rangle = 5, \ \ \ \ \langle \mathbf{v}, \mathbf{w} \rangle  = 0

$$

$$
\lVert \mathbf{u} \rVert = 1, \ \ \ \ \lVert \mathbf{v} \rVert = \sqrt{3}, \ \ \ \ \lVert \mathbf{w} \rVert = 2. 
$$

Evaluate the expression $\langle 2 \mathbf{v} - \mathbf{w}, 3 \mathbf{u} + 2\mathbf{w} \rangle$.
We can separate this out to be
$$
\begin{align}
\left< 2v-w,3u  \right> +\left< 2v-w,2w \right>  
&= 3\left<2v-w,u  \right> +2\left< 2v-w,w \right>  \\
&=3\left< 2v,u \right> +3\left< -w,u \right> +2\left< 2v,w \right> +2\left< -w,w\right>  \\
&=6\left< v,u \right> -3\left< w,u \right> +4\left< v,w \right> -2\left< w,w \right>  \\
&=6(1)-3(5)+4(0)-2(4) \\
&=6-15-8 \\
&=-17
\end{align}
$$



These properties hold because the inner product is
* Symmetric: 
	* $\left< \vec{u},\vec{v} \right> = \left< \vec{v},\vec{u} \right>$
	* $\left< \vec{u},\vec{v}+\vec{w} \right> = \left< \vec{u},\vec{v} \right>+\left< \vec{u},\vec{w} \right>$
* Linear:
	* $\left< c\vec{u},\vec{v} \right> = c\left<\vec{u},\vec{v}  \right>$
* Positive semi-definite:
	* $\left< \vec{u},\vec{v} \right> \geq 0$ with $\left< \vec{u},\vec{u} \right> =0$  if and only if $\vec{u}=\vec{0}$.

