  
## 6.6.32 
  If possible, find a basis $\mathcal{C}$ for $\mathbb{R}^2$ such that the matrix $[T]_\mathcal{C}$ of $T$ with respect to $\mathcal{C}$ is diagonal, where
$$
\begin{align}
T: \mathbb{R}^2 \to \mathbb{R}^2 \text{ defined by } T\begin{bmatrix*}[r] a\\ b \end{bmatrix*} = \begin{bmatrix*}[r] a-b \\ a+b \end{bmatrix*} 
\end{align}
$$

## 7.1.1
Determine which of the four inner product axioms do not hold.
Give a specific example in each case.

Let $\mathbf{u} = \begin{bmatrix*}[r] u_1 \\ u_2 \end{bmatrix*}$ and $\mathbf{v} = \begin{bmatrix*}[r] v_1 \\ v_2 \end{bmatrix*}$ in $\mathbb{R}^2$.
Define $\langle\mathbf{u},\mathbf{v}\rangle = u_1 v_1 -  u_2 v_2$.

The axioms are:
* 〈 u, v〉 = 〈v, u〉 (symmetry axiom)
 We can check if this holds:
$$
\begin{align}
\left< u,v \right> \stackrel{?}{=}  \left< v,u \right>  \\
u_{1}v_{1}-u_{2}v_{2}\stackrel{?}{=}  v_{1}u_{1}-v_{2}u_{2} \\
u_{1}v_{1}-u_{2}v_{2} \stackrel{?}{=}   u_{1}v_{1}-u_{2}v_{2} \\
0 = 0
\end{align}
$$
So the first axiom works.
* 〈u + v, w〉 = 〈u, w〉 + 〈v, w〉 (additivity axiom)
We can check this:
$$
\begin{align}
\left< u+v,w \right> &\stackrel{?}{=}  \left< u,w \right> +\left< v,w \right>  \\
(u_{1}+v_{1})(w_{1})-(u_{2}+v_{2})(w_{2})&\stackrel{?}{=}  u_{1}w_{1}-u_{2}w_{2}+v_{1}w_{1}-v_{2}w_{2} \\
u_{1}w_{1}+v_{1}w_{1}-u_{2}w_{2}-v_{2}w_{2}&\stackrel{?}{=}u_{1}w_{1}-u_{2}w_{2}+v_{1}w_{1}-v_{2}w_{2} \\
0&=0  
\end{align}
$$
So this axiom holds.

*  〈ku, v〉 = k$\left< u, v \right>$ (homogeneity axiom) 
We can check:
$$
\begin{align}
\left< ku,v \right>  & \stackrel{?}{=}  k\left< u,v \right>  \\
(ku_{1})v_{1}-(ku_{2})v_{2} & \stackrel{?}{=}  k(u_{1}v_{1}-u_{2}v_{2}) \\
k(u_{1}v_{1}-u_{2}v_{2})  & \stackrel{?}{=}  k(u_{1}v_{1}-u_{2}v_{2})  \\
0=0
\end{align}
$$
So this holds.
* 〈v, v〉 ≥ 0 and 〈v, v〉 = 0 if and only if v = 0 (positivity axiom)
$$
\begin{align}
\left< v,v \right> \stackrel{?}{>} 0,\text{ for all nonzero v }\\
v_{1}v_{1}-v_{2}v_{2} \stackrel{?}{>}0 \\ \\
\text{ let }v_{1}=2,v_{2}=2. \\
2*2-2*2=0
\end{align}
$$
With a nonzero input vector $v=(2,2)$, the inner product yields zero. Because it must hold that an inner product equals zero if and only if $v=\vec{0}$, this axiom does not hold true.




## 7.1.4

Apply the Gram--Schmidt Process to the basis $\mathcal{B}$ to obtain an orthogonal basis for the inner product space $V$ relative to the given inner product.

Let $V = \mathscr{P}_2[0,1]$, $\mathcal{B} = \left\{1, 1+x, 1+x+x^2\right\}$, with the inner product in Example 7.5.
$$
\begin{align}
\left< f,g \right> =\int_{0}^{1} f(x)g(x) \, dx 
\end{align}
$$
We pick an arbitrary vector as the first for our orthogonal set:
$$
\begin{align}
v_{1}=b_{1}=1
\end{align}
$$
Now applying gram Schmidt,
$$
\begin{align}
v_{2} & =b_{2}-\frac{\left< v_{1},b_{2} \right>}{\left< v_{1},v_{1} \right> }b_{1}  \\
v_{2} & =1+x-\frac{\left( \int_{0}^{1} (1)(1+x) \, dx  \right)}{\left( \int_{0}^{1} (1)(1) \, dx  \right)} \\
v_{2} & =1+x-\frac{\left( x+\frac{x^{2}}{2} \right)\bigg|_{0}^{1}}{x\bigg|_{0}^{1}  }   \\
v_{2} & =1+x-\frac{\left( 1+\frac{1}{2} \right)}{1} \\
v_{2}  & =1+x-\frac{3}{2} \\
v_{2} & = x-\frac{1}{2}
\end{align}
$$
Next, to find $v_{3}:$
$$
\begin{align}
v_{3}=b_{3}-\frac{\left< v_{1},b_{3} \right> }{\left< v_{1},v_{1} \right> }v_{1}- \frac{\left< v_{2},b_{3} \right> }{\left< v_{2},v_{2} \right> }v_{2} \\
v_{3}=b_{3}-\left( \int_{0}^{1} 1+x+x^{2} \, dx  \,  \right)(1)- \frac{\int_{0}^{1} \left( x-\frac{1}{2} \right)(1+x+x^{2}) \, dx }{\int_{0}^{1} \left( x-\frac{1}{2} \right)^{2} \, dx }(1+x) \\
v_{3}=b_{3}-\left( 1+\frac{1}{2}+\frac{1}{3} \right)-\frac{\int_{0}^{1} x-\frac{1}{2}+x^{2}-\frac{1}{2}x+x^{3}-\frac{1}{2}x^{2} \, dx }{\int_{0}^{1} x^{2}-x+\frac{1}{4} \, dx } \\
v_{3}=b_{3}-\left( \frac{11}{6} \right)-\frac{\frac{1}{2}-\frac{1}{2}+\frac{1}{3}-\frac{1}{4}+\frac{1}{4}-\frac{1}{6}}{\frac{1}{3}-\frac{1}{2}+\frac{1}{4}} \\ \\
v_{3}=b_{3}-\frac{11}{6}-\frac{\left( \frac{1}{6} \right)}{\frac{1}{12}}\\
v_{3}=b_{3} -\frac{11}{6}-2\\
v_{3} = 1+x+x^{2}-\left( \frac{11}{6}+\frac{12}{6} \right) \\
v_{3}=\frac{28}{6}+x+x^{2}
\end{align}
$$

This gives us $\left\{ \frac{28}{6}+x+x^{2},x-\frac{1}{2},1 \right\}$ as an orthogonal basis.




 If possible, find a basis $\mathcal{C}$ for $\mathbb{R}^2$ such that the matrix $[T]_\mathcal{C}$ of $T$ with respect to $\mathcal{C}$ is diagonal, where
$$
\begin{align}
T: \mathbb{R}^2 \to \mathbb{R}^2 \text{ defined by } T\begin{bmatrix*}[r] a\\ b \end{bmatrix*} = \begin{bmatrix*}[r] a-b \\ a+b \end{bmatrix*}
\end{align}
$$
To find this, we need the transformed version of each element in the basis to form a diagonal matrix when all glued together.

Thus,
