## 6.4.18

Let $T: M_{22} \to \mathbb{R}$ be a linear transformation for which
$$

    \begin{align*}
        T\begin{bmatrix*} 1 & 0 \\ 0 & 0 \end{bmatrix*} &= 1, \\
        T\begin{bmatrix*} 1 & 1 \\ 0 & 0 \end{bmatrix*} &= 2, \\
        T\begin{bmatrix*} 1 & 1 \\ 1 & 0 \end{bmatrix*} &= 3, \text{ and } \\
        T\begin{bmatrix*} 1 & 1 \\ 1 & 1 \end{bmatrix*} &= 4.
    \end{align*}
$$

Find $T\begin{bmatrix*}[r] 1 & 3 \\ 4 & 2 \end{bmatrix*}$ and $T\begin{bmatrix*}[r] a & b \\ c & d \end{bmatrix*}$.

First, we must assert that 
$$
\left\{  
\begin{bmatrix*} 1 & 0 \\ 0 & 0 \end{bmatrix*} ,
\begin{bmatrix*} 1 & 1 \\ 0 & 0 \end{bmatrix*}, 
\begin{bmatrix*} 1 & 1 \\ 1 & 0 \end{bmatrix*}, 
\begin{bmatrix*} 1 & 1 \\ 1 & 1 \end{bmatrix*}
\right\}
$$
is a basis for every two by two matrix. We can check this by multiplying by constants $c_{1}\dots c_{4}$, summing across all of them, and seeing if the result can reach all of $M_{2,2}$
This is
$$
\begin{bmatrix}
c_{1}+c_{2}+c_{3}+c_{4} & c_{2}+c_{3}+c_{4} \\
c_{3}+c_{4} & c_{4}
\end{bmatrix}
$$
We have four independent equations, and can uniquely specify all of $M_{2,2}$. 

We can thus represent the transformation as
$$
c_{1}\begin{bmatrix*} 1 & 0 \\ 0 & 0 \end{bmatrix*} +c_{2}
\begin{bmatrix*} 1 & 1 \\ 0 & 0 \end{bmatrix*}+c_{3} 
\begin{bmatrix*} 1 & 1 \\ 1 & 0 \end{bmatrix*} +c_{4} 
\begin{bmatrix*} 1 & 1 \\ 1 & 1 \end{bmatrix*} = \begin{bmatrix}
1 & 3 \\ 4 & 2
\end{bmatrix}
$$
This reduces to the problem:
$$
\begin{bmatrix}
1 & 1 & 1 & 1 & | & 1 \\
0 & 1 & 1 & 1 & | & 3 \\
0 & 0 & 1 & 1 & | & 4 \\
0 & 0 & 0 & 1 & | & 2
\end{bmatrix}
$$
Thus, $c_{4}=2,c_{3}=2,c_{2}=-1,c_{1}=-2$
Therefore,
$T\begin{bmatrix*}[r] 1 & 3 \\ 4 & 2 \end{bmatrix*}=$
$$
T \left( -2 \begin{bmatrix*} 1 & 0 \\ 0 & 0 \end{bmatrix*} -1
\begin{bmatrix*} 1 & 1 \\ 0 & 0 \end{bmatrix*}+2
\begin{bmatrix*} 1 & 1 \\ 1 & 0 \end{bmatrix*} +2
\begin{bmatrix*} 1 & 1 \\ 1 & 1 \end{bmatrix*} = \begin{bmatrix}
1 & 3 \\ 4 & 2
\end{bmatrix} \right) 
$$
$$
= 
-2T\begin{bmatrix*} 1 & 0 \\ 0 & 0 \end{bmatrix*} -1T
\begin{bmatrix*} 1 & 1 \\ 0 & 0 \end{bmatrix*}+2T
\begin{bmatrix*} 1 & 1 \\ 1 & 0 \end{bmatrix*} +2T
\begin{bmatrix*} 1 & 1 \\ 1 & 1 \end{bmatrix*} = T\begin{bmatrix}
1 & 3 \\ 4 & 2
\end{bmatrix}
$$
This reduces to
$$
\begin{align}
-2 (1) - 1 (2) + 2(3) + 2 (4) \\
= -2-2+6+8 \\
\end{align}
$$
$$
\boxed{
T\begin{bmatrix*}[r] 1 & 3 \\ 4 & 2 \end{bmatrix*}=10
}
$$

We can do the same for
$$
\begin{bmatrix}
a & b \\ c & d
\end{bmatrix}
$$
$$
\begin{bmatrix}
1 & 1 & 1 & 1 & | & a \\
0 & 1 & 1 & 1 & | & b \\
0 & 0 & 1 & 1 & | & c \\
0 & 0 & 0 & 1 & | & d
\end{bmatrix}
$$

$$
\begin{align}
c_{4} = d \\
c_{3}=c-c_{4} \\
=c-d \\
c_{2}=b-c_{3}-c_{4} \\
=b-c+d-d \\
=b-c\\ \\
c_{1}=a-c_{2}-c_{3}-c_{4} \\
=a-b+c-c+d-d \\
=a-b
\end{align}
$$
Now that we have the constants:
$$\begin{align}
c_{1}= a-b, \\
c_{2}=b-c \\
c_{3}=c-d \\
c_{4}=d
\end{align}
$$
We can solve:
$$
= 
c_{1}T\begin{bmatrix*} 1 & 0 \\ 0 & 0 \end{bmatrix*} 
+c_{2}T
\begin{bmatrix*} 1 & 1 \\ 0 & 0 \end{bmatrix*}+c_{3}
\begin{bmatrix*} 1 & 1 \\ 1 & 0 \end{bmatrix*} +c_{4}
\begin{bmatrix*} 1 & 1 \\ 1 & 1 \end{bmatrix*} = \begin{bmatrix}
1 & 3 \\ 4 & 2
\end{bmatrix}
$$
$$
= (a-b)T\begin{bmatrix*} 1 & 0 \\ 0 & 0 \end{bmatrix*} 
+(b-c)T
\begin{bmatrix*} 1 & 1 \\ 0 & 0 \end{bmatrix*}+(c-d)
\begin{bmatrix*} 1 & 1 \\ 1 & 0 \end{bmatrix*} +(d)
\begin{bmatrix*} 1 & 1 \\ 1 & 1 \end{bmatrix*}
$$
$$
\begin{align}
(a-b) (1) +(b-c) (2) + (c-d)(3) + d (4) \\
= a-b+2b-2c+3c-3c+4d \\
=a+b+c+d
\end{align}
$$

$$
\boxed{
T\begin{bmatrix}
a & b\\ c & d
\end{bmatrix} = a+b+c+d
}
$$

## 6.4.20
$$
\text{ Show that there is no linear transformation $T:\mathbb{R}^{3}\rightarrow \mathscr{P}_2$ such that  }
$$

$$
\begin{align*}
        T\begin{bmatrix*}[r] 2 \\ 1 \\ 0 \end{bmatrix*} &= 1 + x, \\
        T\begin{bmatrix*}[r] 3 \\ 0 \\ 2 \end{bmatrix*} &= 2 - x + x^2, \text{ and} \\
        T\begin{bmatrix*}[r] 0 \\ 6 \\ -8 \end{bmatrix*} &= -2 + 2x^2. 
    \end{align*}
$$
This transformation must be linear, meaning it has to satisfy 
$T(\vec{u}+\vec{v})=T(\vec{u})+T(\vec{v})$ and $T(c\vec{u})=cT(\vec{u})$

First, I'll check if these values are linearly independent to see if the construction involves a contradiction with one of the outputs.
$$
\begin{bmatrix}
2 & 3 & 0 \\
1 & 0 & 6 \\
0 & 2 & -8
\end{bmatrix}
$$
$$
\begin{bmatrix}
1 & 0 & 6 \\
2 & 3 & 0 \\
0 & 2 & -8
\end{bmatrix} \rightarrow \begin{bmatrix}
1 & 0 & 6 \\
0 & 3 & -12 \\
0 & 2 & -8 
\end{bmatrix}\rightarrow \begin{bmatrix}
1 & 0 & 6 \\
0 & 1 & -4 \\
0 & 1 & -4
\end{bmatrix}\rightarrow \begin{bmatrix}
1 & 0 & 6 \\
0 & 1 & -4 \\
0 & 0 & 0
\end{bmatrix}
$$
We can see that this is not linearly independent. Thus, we can check to see if a linear combination of two vectors will produce the output of the third.
$$
c_{1} \begin{bmatrix}
2 \\ 1 \\ 0
\end{bmatrix} + c_{2} \begin{bmatrix}
3 \\ 0 \\ 2
\end{bmatrix} = \begin{bmatrix}
0 \\ 6 \\ -8
\end{bmatrix}
$$
This simplifies to
$$
\begin{bmatrix}
2 & 3 & | & 0 \\
1 & 0 & | & 6 \\
0 & 2 & | & -8
\end{bmatrix}
$$
We can see easily that $c_{2}=-4$ and $c_{1}=6$. 
We can check the first equality by $2(6)+3(-4)=0$, $12-12=0,0=0$ which is true. Thus, we can check if the output of the third is the linear combination of the outputs of the first two transformations:
$$
\begin{align}
6 T\begin{bmatrix}
2 \\ 1 \\ 0
\end{bmatrix} - 4 T\begin{bmatrix}
3 \\ 0 \\ 2
\end{bmatrix} \stackrel{?}{=} T\begin{bmatrix}
0 \\ 6 \\ -8
\end{bmatrix} \\
6(1+x)-4(2-x+x^{2})\stackrel{?}{=} -2+2x^{2} \\
6+6x-8+4x-4x^{2}\stackrel{?}{=} -2+2x^{2} \\
-4x^{2}+10x-2 \neq -2+2x^{2}
\end{align}
$$
Therefore, there is no **LINEAR** transformation $T$ that holds the properties above. The third function is not a linear transformation of the other two, despite being in the span of the other two.


## 6.4.26

Define linear transformations $S: \mathscr{P}_1 \to \mathscr{P}_2$ and $T: \mathscr{P}_2 \to \mathscr{P}_1$ by
$$
    S(a+bx) = a + (a+b)x + 2bx^2
        \text{ \ and \ }
        T(a+bx+cx^2) = b + 2cx. 

$$
Compute $(S \circ T)(3 + 2x - x^2)$ and $(S \circ T)(a + bx + cx^2)$.
Can you compute $(T \circ S)(a + bx)$? If so, compute it.

The composition $(S\circ T)\vec{u}=S(T(\vec{u}))$ by definition.

1) The first problem
$$
\begin{align}
(S \circ T)(3 + 2x - x^2) \\
= S(T(3 + 2x - x^2)) \\
\end{align}
$$
We can find the inner first: 
$$
\begin{align}
T(3 + 2x - x^{2)}= (2) + 2(-1)x \\
= 2-2x
\end{align}
$$
Now the outer, $S(2-2x)$
$$
\begin{align}
S(2-2x)=2 +(2-2)x+2(-2)x^{2}
\end{align}
$$
Thus,
$$
S(T(3+2x^{2}-x^{2})) =2-4x^{2}
$$



2) The second problem:

$$
\begin{align}
(S \circ T)(a + bx + cx^2) \\
= S(T(a+bx+cx^{2})) \\
=S(b+2cx) \\
= b+(b+2c)x+2(2c)x^{2} \\
= b +bx+2cx+4cx^{2}
\end{align}
$$

3)  compute $(T \circ S)(a + bx)$. Note that $T$ and $S$ switched places. We can compute, because dimensions match the requirement to apply each transformation.
This simplifies to 
$$
\begin{align}
T(S(a+bx)) = T(a+(a+b)x+2bx^{2}) \\
= (a+b)+2(2b)x \\
= a+b+4bx
\end{align}
$$


## 6.5.2
 Let $T: M_{22} \to \mathbb{R}$ be the linear transformation defined by $T(A) = \text{tr}(A)$.

Which, if any, of the following matrices are in $\text{ker}(T)$?
$$
    \text{\textbf{(i)}} \begin{bmatrix*}[r] 1 & 2 \\ -1 & 3 \end{bmatrix*}
                \text{ \ \ \ \ \ \ \ }
                \text{\textbf{(ii)}} \begin{bmatrix*} 0 & 4 \\ 2 & 0 \end{bmatrix*}
                \text{ \ \ \ \ \ \ \ }
                \text{\textbf{(iii)}} \begin{bmatrix*}[r] 1 & 3 \\ 0 & -1 \end{bmatrix*}
$$

$Ker(T) = \left\{ A : T(A)=0 \right\}$
$tr(i)=3$, $tr(ii)=0,tr(iii)=0$

Thus, ii and iii are in the kernel of $T$.

Which, if any, of the following scalars are in $\text{range}(T)$?

$$
\text{\textbf{(i)} } 0
\text{ \ \ \ \ \ \ \ }
\text{\textbf{(ii)} } 2
\text{ \ \ \ \ \ \ \ }
\text{\textbf{(iii)} } \frac{\sqrt{2}}{2}

$$
All three are in the range of $T$, for example:
$$
T(\begin{bmatrix}
0 & 1 \\
1 & 0
\end{bmatrix})= 0, 
T(\begin{bmatrix}
1 & 0 \\
0 & 1
\end{bmatrix})=2,
T\left( \begin{bmatrix}
\frac{\sqrt{ 2 }}{2}-1,0 \\
0 & 1
\end{bmatrix} \right)=\frac{\sqrt{ 2 }}{2}
$$

Describe $\text{ker}(T)$ and $\text{range}(T)$.
The kernel of $T$ is
$$
\begin{align}
\left\{ A:T(A)=0 \right\} \\
\implies \left\{ \begin{bmatrix}
a & b \\ c & d
\end{bmatrix}: a+d=0 \ \ \ \forall \ \ a,b,c,d \in   \mathrm{Re} \right\}
\end{align}
$$




## 6.5.4
Let $T: \mathscr{P}_2 \to \mathscr{P}_2$ be the linear transformation defined by $T(p(x)) = xp'(x)$.
*This is worded poorly, as i initially interpreted this as (input)x(derivative of input, which leaves the set for p(x) = x^2)*

Which, if any, of the following polynomials are in $\text{ker}(T)$?
$$
\text{\textbf{(i)} } 1
\text{ \ \ \ \ \ \ \ }
\text{\textbf{(ii)} } x
\text{ \ \ \ \ \ \ \ }
\text{\textbf{(iii)} } x^2
$$
1) $T(1)=1\left( \frac{d}{dt}1 \right)=0x=0$. Thus,  $1$ is in $ker(T)$
2) $T(x)=x\left( \frac{d}{dt}x \right)=1x=x$ So $x$ is not in $ker(T)$
3) $T(x^{2})=x\frac{dx^{2}}{dx}=x(2x)=2x^{2}$, so $x^{2}$ is not in $ker(T)$. However, this has left the set, as $x^{3}$ is not in $\mathscr{P}_{2}$. 

Which, if any, of the polynomials from part (a) are in $\text{range}(T)$?
By the rank-nullity theorem,
 $x,x^{2}$ are the only one in $range(T)$. 

Describe $\text{ker}(T)$ and $\text{range}(T)$.

$Ker(T)=$
$$
\begin{align}
\left\{ xp'(x)=0 \right\} \\
\implies p'(x)=0 \text{ or }  x=0\\
\implies \left\{ x \in  (c_{1} , 0 , 0)\begin{bmatrix}
1 \\ x\\ x^{2}
\end{bmatrix} \forall c_{1} \right\}
\end{align}
$$

The kernel of $T$ is every polynomial in $\mathscr{P}_{2}: c_{1}x+c_{2}x^{2}+c_{3}x^{3}$ where $c_{2}=c_{3}=0$ 
The $Range$ of $T$ is every polynomial is $\mathscr{P}_{2}$:
$$
\left\{ bx+cx^{2}:b,c \in  \mathrm{Re} \right\}
$$as the derivative of a constant is zero, and x(0) = 0, so there is no constant term. 
